VeriTile/Triton/DSL/Metadata.lean
@@ -354,12 +354,9 @@ private partial def stmtRegionsWith (assigned : List String)
   | `(tritonStmt| for $idx:ident in range($($_:term), $($_:term), $($_:term)) { $stmts:tritonStmt* }) =>
       let (i, o, _) := blockRegionsWith (idx.getId.toString :: assigned) stmts.toList
       (i, o, assigned)
-<<<<<<< Updated upstream
-=======
   | `(tritonStmt| for $idx:ident in range($start:tritonExpr, $stop:tritonExpr, $step:tritonExpr) { $stmts:tritonStmt* }) =>
       let (i, o, _) := blockRegionsWith (idx.getId.toString :: assigned) stmts.toList
       (exprRegions assigned start ++ exprRegions assigned stop ++ exprRegions assigned step ++ i, o, assigned)
->>>>>>> Stashed changes
   | `(tritonStmt| tl.static_range $idx:ident in $($_:term) { $stmts:tritonStmt* }) =>
       let (i, o, _) := blockRegionsWith (idx.getId.toString :: assigned) stmts.toList
       (i, o, assigned)
