VeriTile/Triton/Memory/Typing/Checker.lean
@@ -222,15 +222,11 @@ def Op.blockPtrProvenance (ctx : CheckCtx) :
     Op dtype shape → Except CheckError RegionName
   | .makeBlockPtr region _ parentShape blockShape strides offsets => do
       checkBlockPtrMetadata parentShape blockShape strides offsets
-<<<<<<< Updated upstream
       .ok (Region.cast region)
-=======
-      .ok region
   | .makeBlockPtrDyn region base parentShape blockShape strides offsets => do
       base.check ctx
       checkBlockPtrMetadata parentShape blockShape strides offsets
       .ok region
->>>>>>> Stashed changes
   | .advanceBlockPtr ptr _ => ptr.blockPtrProvenance ctx
   | .broadcast ptr _ => ptr.blockPtrProvenance ctx
   | .full _ ptr => ptr.blockPtrProvenance ctx
@@ -321,15 +317,12 @@ def Stmt.check (ctx : CheckCtx) : Stmt → Except CheckError CheckCtx
   | .forRange idx _ _ _ body => do
       let ctx' ← ctx.setReg idx (pointerEntry .nat [] none none)
       StmtList.check ctx' body
-<<<<<<< Updated upstream
-=======
   | .forRangeDyn idx start stop step body => do
       start.check ctx
       stop.check ctx
       step.check ctx
       let ctx' ← ctx.setReg idx (pointerEntry .nat [] none none)
       StmtList.check ctx' body
->>>>>>> Stashed changes
   | .ifThen cond body => do
       cond.check ctx
       StmtList.check ctx body
